skip toLayered correctness

CircuitComp/BranchingProgram/Basic.lean
@@ -614,43 +614,101 @@ theorem nonempty_of_depth_pos (h : 0 < P.depth) : Nonempty α :=
   let u : P.nodes z.castSucc := cast (by simp [z]) P.start
   ⟨P.nodeVar u⟩
 
+/-- The "active edges" at layer `i` are the edges that skip past layer `i`. -/
+def ActiveEdges (i : Fin (P.depth + 1)) : Type v :=
+  Σ (l : { l : Fin P.depth // l.castSucc < i }),
+    Σ (u : P.nodes l.val.castSucc), { b : β // (P.edges u b).1 > i }
+
+lemma ActiveEdges_last_isEmpty : IsEmpty (P.ActiveEdges (Fin.last P.depth)) :=
+  ⟨fun ⟨_, h⟩ ↦ not_lt_of_ge (Fin.le_last _) h.2.2⟩
+
 /--
 Conversion from `SkipBranchingProgram` to `LayeredBranchingProgram`.
 Adds dummy nodes to carry values across skipped layers.
 -/
-def toLayeredBranchingProgram : LayeredBranchingProgram α β γ where
+def toLayered : LayeredBranchingProgram α β γ where
   depth := P.depth
-  nodes i := (P.nodes i) ⊕ Σ (j : Fin P.depth.succ), { v : P.nodes j // j > i ∧ i.val > 0 }
+  nodes i := P.nodes i ⊕ P.ActiveEdges i
   nodeVar {i} u := match u with
     | .inl u => P.nodeVar u
     | .inr _ =>
       if h : Nonempty (P.nodes i.castSucc) then
         P.nodeVar (Classical.choice h)
       else
-        (P.nonempty_of_depth_pos (by linarith [i.2])).some
-  edges {i} u b := match u with
+        (P.nonempty_of_depth_pos (lt_of_le_of_lt (Nat.zero_le _) i.isLt)).some
+  edges {i} node val := match node with
     | .inl u =>
+      let next := P.edges u val
+      let m := next.1
+      let v := next.2
+      if h : m = i.succ then
+        .inl (h ▸ v)
+      else
+        .inr ⟨⟨i, Fin.castSucc_lt_succ i⟩, ⟨u, ⟨val, lt_of_le_of_ne (Nat.succ_le_of_lt (P.edges_layer_gt u val)) (Ne.symm h)⟩⟩⟩
+    | .inr ⟨⟨l, hl⟩, u, ⟨b, hb⟩⟩ =>
       let next := P.edges u b
       let m := next.1
       let v := next.2
       if h : m = i.succ then
         .inl (h ▸ v)
       else
-        .inr ⟨m, ⟨v, ⟨lt_of_le_of_ne (P.edges_layer_gt u b) (Ne.symm h), i.succ_pos⟩⟩⟩
-    | .inr ⟨m, ⟨v, ⟨hm, _⟩⟩⟩ =>
-      if h : m = i.succ then
-        .inl (h ▸ v)
-      else
-        .inr ⟨m, ⟨v, ⟨lt_of_le_of_ne (Nat.succ_le_of_lt hm) (Ne.symm h), i.succ_pos⟩⟩⟩
+        .inr ⟨⟨l, lt_trans hl (Fin.castSucc_lt_succ i)⟩, ⟨u, ⟨b, lt_of_le_of_ne (Nat.succ_le_of_lt hb) (Ne.symm h)⟩⟩⟩
   startUnique := {
     default := .inl P.start
     uniq u := by
-      cases u
+      rcases u with _ | ⟨⟨l, hl⟩, _⟩
       · simpa using P.startUnique.uniq _
-      · aesop
+      · exact (Nat.not_lt_zero _ hl).elim
   }
   retVals u := match u with
     | .inl u => P.retVals u
-    | .inr ⟨_, ⟨_, ⟨h, _⟩⟩⟩ => (h.not_ge (Fin.le_last _)).elim
+    | .inr ⟨_, ⟨_, ⟨_, hb⟩⟩⟩ => (Nat.not_lt_of_le (Fin.le_last _) hb).elim
+
+theorem toLayered_evalAt
+      (x : α → β) (i : Fin (P.depth + 1)) (node : P.toLayered.nodes i) :
+    (P.toLayered).evalAt x i node =
+    match node with
+    | .inl u => P.evalAt x u
+    | .inr ⟨_, u, b, _⟩ => P.evalAt x (P.edges u b).2 := by
+  have h_ind : ∀ j : Fin (P.depth + 1), ∀ node, (P.toLayered).evalAt x j node = match node with
+    | .inl u => P.evalAt x u
+    | .inr ⟨fst, ⟨u, ⟨b, property⟩⟩⟩ => P.evalAt x (P.edges u b).snd := by
+    intro j;
+    induction' j using Fin.reverseInduction with j ih;
+    · intro node
+      cases' node with u hu;
+      · unfold SkipBranchingProgram.toLayered LayeredBranchingProgram.evalAt;
+        simp [ Fin.ext_iff, SkipBranchingProgram.evalAt ] at *;
+      · exact False.elim <| P.ActiveEdges_last_isEmpty.elim hu;
+    · intro node;
+      convert ih ( ( P.toLayered ).edges node ( x ( ( P.toLayered ).nodeVar node ) ) ) using 1;
+      · rw [ LayeredBranchingProgram.evalAt ];
+        simp [ Fin.ext_iff];
+        exact fun h => False.elim <| h.not_lt <| Fin.is_lt j;
+      · cases node <;> simp [ SkipBranchingProgram.toLayered ];
+        · split_ifs <;> simp [ * ];
+          · rw [ SkipBranchingProgram.evalAt ];
+            simp [ Fin.ext_iff];
+            grind;
+          · rw [ SkipBranchingProgram.evalAt ];
+            simp [ Fin.ext_iff];
+            exact fun h => absurd h ( ne_of_lt j.2 );
+        · cases' ‹P.ActiveEdges j.castSucc› with l hl;
+          grind;
+  exact h_ind _ _
+
+open Classical in
+@[simp]
+theorem toLayered_eval : P.toLayered.eval = P.eval := by
+  have h_eval_eq (x) : P.toLayered.eval x = P.toLayered.evalAt x 0 P.toLayered.start := by
+    rw [LayeredBranchingProgram.eval]
+    convert P.toLayered.evalAt_evalLayer_eq_eval x (Fin.last _) using 1
+    · unfold LayeredBranchingProgram.evalAt
+      simp
+    · rw [← LayeredBranchingProgram.evalAt_evalLayer_eq_eval]
+      rfl
+  ext1
+  rw [h_eval_eq, toLayered_evalAt]
+  rfl
 
 end SkipBranchingProgram
